using assume type instead of opaque type for types with no defn., fixing proofs with the change

examples/wysteria/crypto.fst
@@ -1,5 +1,5 @@
 (*--build-config
-    options:--admit_fsi FStar.OrdSet --admit_fsi FStar.OrdMap --admit_fsi FStar.Set --admit_fsi Ffibridge --admit_fsi FStar.Seq  --admit_fsi Runtime --admit_fsi FStar.IO --admit_fsi FStar.String --__temp_no_proj PSemantics;
+    options:--admit_fsi FStar.OrdSet --admit_fsi FStar.OrdMap --admit_fsi FStar.Set --admit_fsi Ffibridge --admit_fsi FStar.Seq  --admit_fsi Runtime --admit_fsi FStar.IO --admit_fsi FStar.String --__temp_no_proj PSemantics --verify_module Crypto;
     variables:CONTRIB=../../contrib;
     other-files:classical.fst ext.fst set.fsi heap.fst st.fst all.fst seq.fsi seqproperties.fst ghost.fst listTot.fst ordset.fsi ordmap.fsi list.fst io.fsti string.fst prins.fst ast.fst ffibridge.fsi sem.fst psem.fst $CONTRIB/Platform/fst/Bytes.fst runtime.fsi print.fst $CONTRIB/CoreCrypto/fst/CoreCrypto.fst ../crypto/sha1.fst
  --*)
@@ -69,8 +69,8 @@ let verify_mac (#a:Type) (#key_prop:key -> a -> Type) k m t =
   if (not b) then None
   else Some (unmarshal #a m)
 
-opaque type client_key_prop: key -> (prin * redex) -> Type
-opaque type server_key_prop: key -> server_ret_type -> Type
+assume type client_key_prop: key -> (prin * redex) -> Type
+assume type server_key_prop: key -> server_ret_type -> Type
 
 type client_key = k:key{client_key_prop k == client_prop_t}
 type server_key = k:key{server_key_prop k == server_prop_t}
